Current

lean/language.lean
@@ -17,19 +17,87 @@ namespace IncLoLang
 
 meta def tactic.dec_trivial := `[exact dec_trivial]
 
-def state : Type := string × ℕ -> Prop
+-- def state : Type := string × ℕ -> Prop
+
+-- def state.update : string -> ℕ -> state -> state
+-- | name val s := (λ pair, pair == (name, val) ∨ s pair)
+
+-- notation s `{` name ` ↦ ` val `}` := state.update name val s
+
+-- @[simp] lemma update_apply (name : string) (val : ℕ) (s : state) :
+--   s{name ↦ val} (name, val) :=
+-- begin
+--   unfold state.update,
+--   finish,
+-- end
+
+-- @[simp] lemma repeat (name : string) (val : ℕ) (s : state) :
+--   s{name ↦ val}{name ↦ val} = s{name ↦ val} :=
+-- begin
+--   unfold state.update,
+--   finish,
+-- end
+
+def state: Type := string -> ℕ
 
 def state.update : string -> ℕ -> state -> state
-| name val s := (λ pair, pair == (name, val) ∨ s pair)
+| name val σ := (λ name', if name' = name then val else σ name')
 
 notation s `{` name ` ↦ ` val `}` := state.update name val s
 
-@[simp] lemma update_apply (name : string) (val : ℕ) (s : state) :
-  s{name ↦ val} (name, val) :=
+@[simp] lemma state.update_apply (name : string) (val : ℕ) (s : state) :
+  s{name ↦ val} name = val :=
 begin
   unfold state.update,
   finish,
 end
+
+lemma test :
+  (if ff then 1 else 2) = 2 :=
+begin
+  exact if_neg (bool.not_ff),
+end
+
+@[simp] lemma update_apply_ne (name name' : string) (val : ℕ) (s : state)
+    (h : name' ≠ name) :
+  s{name ↦ val} name' = s name' :=
+begin
+  unfold state.update,
+  exact if_neg h,
+end
+
+@[simp] lemma update_override (name : string) (val₁ val₂ : ℕ) (s : state) :
+  s{name ↦ val₂}{name ↦ val₁} = s{name ↦ val₁} :=
+begin
+  apply funext,
+  intro name',
+  by_cases name' = name;
+    simp [h]
+end
+
+@[simp] lemma update_swap (name₁ name₂ : string) (val₁ val₂ : ℕ) (s : state)
+    (h : name₁ ≠ name₂ . tactic.dec_trivial) :
+  s{name₂ ↦ val₂}{name₁ ↦ val₁} = s{name₁ ↦ val₁}{name₂ ↦ val₂} :=
+begin
+  apply funext,
+  intro name',
+  by_cases name' = name₁;
+    by_cases name' = name₂;
+    simp * at *
+end
+
+@[simp] lemma update_id (name : string) (s : state) :
+  s{name ↦ s name} = s :=
+begin
+  apply funext,
+  intro name',
+  by_cases name' = name;
+    simp * at *
+end
+
+@[simp] lemma update_same_const (name : string) (val : ℕ) :
+  (λ_, val){name ↦ val} = (λ_, val) :=
+by apply funext; simp
 
 /-! ## Language -/
 
